Fixed the refactoring

Source/DafnyCore/AST/Tokens.cs
@@ -44,7 +44,6 @@ public interface IToken : Microsoft.Boogie.IToken {
   /// ```
   /// </summary>
   string TrailingTrivia { get; set; }
-
   string LeadingTrivia { get; set; }
   IToken Next { get; set; } // The next token
   IToken Prev { get; set; } // The previous token
