Source/DafnyCore/GeneratedFromDafny.cs
@@ -1,42 +1,54 @@
-/// Microsoft.Dafny.Formatting.__default.ReindentProgramFromFirstToken() takes
-/// - A first token, from which an entire program is available
-/// - An IIndentationFormatter, that knows how to indent every token
-/// It then prints every token (proven separatedly) in order, reindenting its leading trivia and trailing trivia
+// Dafny program Formatting.dfy compiled into C#
+// To recompile, you will need the libraries
+//     System.Runtime.Numerics.dll System.Collections.Immutable.dll
+// but the 'dotnet' tool in net6.0 should pick those up automatically.
+// Optionally, you may want to include compiler switches like
+//     /debug /nowarn:162,164,168,183,219,436,1717,1718
 
 using System;
 using System.Numerics;
 using System.Collections;
-using System.Text;
-using Microsoft.Dafny;
-
 namespace Formatting {
 
   public interface IIndentationFormatter {
-    string GetNewLeadingTrivia(IToken token);
-    string GetNewTrailingTrivia(IToken token);
-    void GetNewLeadingTrailingTrivia(IToken token, out string newLeadingTrivia, out string newTrailingTrivia);
+    System.String GetNewLeadingTrivia(Microsoft.Dafny.IToken token);
+    System.String GetNewTrailingTrivia(Microsoft.Dafny.IToken token);
+    void GetNewLeadingTrailingTrivia(Microsoft.Dafny.IToken token, out System.String newLeadingTrivia, out System.String newTrailingTrivia);
   }
   public class _Companion_IIndentationFormatter {
-    public static void GetNewLeadingTrailingTrivia(
-        IIndentationFormatter _this, IToken token,
-        out string newLeadingTrivia, out string newTrailingTrivia) {
-      newLeadingTrivia = _this.GetNewLeadingTrivia(token);
-      newTrailingTrivia = _this.GetNewTrailingTrivia(token);
+    public static void GetNewLeadingTrailingTrivia(Formatting.IIndentationFormatter _this, Microsoft.Dafny.IToken token, out System.String newLeadingTrivia, out System.String newTrailingTrivia) {
+      newLeadingTrivia = default(System.String);
+      newTrailingTrivia = default(System.String);
+      newLeadingTrivia = (_this).GetNewLeadingTrivia(token);
+      newTrailingTrivia = (_this).GetNewTrailingTrivia(token);
     }
   }
 
-  public class __default {
-    public static string ReindentProgramFromFirstToken(IToken firstToken, IIndentationFormatter reindent) {
-      var token = firstToken;
-      var sb = new StringBuilder();
-      while (token != null) {
-        reindent.GetNewLeadingTrailingTrivia(token, out var newLeadingTrivia, out var newTrailingTrivia);
-        sb.Append(newLeadingTrivia);
-        sb.Append(token.val);
-        sb.Append(newTrailingTrivia);
+  public partial class __default {
+    public static System.String ReindentProgramFromFirstToken(Microsoft.Dafny.IToken firstToken, Formatting.IIndentationFormatter reindent) {
+      System.String s = default(System.String);
+      Microsoft.Dafny.IToken token;
+      token = firstToken;
+      System.Text.StringBuilder sb;
+      System.Text.StringBuilder _nw0 = new System.Text.StringBuilder();
+      sb = _nw0;
+      while ((token) != (object)((Microsoft.Dafny.IToken)null)) {
+        System.String newLeadingTrivia;
+        System.String newTrailingTrivia;
+        System.String _out0;
+        System.String _out1;
+        (reindent).GetNewLeadingTrailingTrivia(token, out _out0, out _out1);
+        newLeadingTrivia = _out0;
+        newTrailingTrivia = _out1;
+        (sb).Append(newLeadingTrivia);
+        (sb).Append(token.val);
+        (sb).Append(newTrailingTrivia);
         token = token.Next;
       }
-      return sb.ToString();
+      System.String _out2;
+      _out2 = (sb).ToString().ToString();
+      s = _out2;
+      return s;
     }
   }
 } // end of namespace Formatting
